TotalSemProperties.thy
@@ -499,12 +499,372 @@ proof cases
     by (metis exhale_state_same_store exhale_state_same_trace \<open>\<omega>' \<in> _\<close>)
 qed
 
-subsection \<open>Relationship inhale and exhale\<close>
-
 lemma exhale_normal_result_smaller:
   assumes "red_exhale ctxt StateCons \<omega>def A \<omega> (RNormal \<omega>')"
   shows "\<omega> \<succeq> \<omega>'"
   sorry
+
+subsection \<open>Relationship inhale and exhale\<close>
+
+lemma red_pure_exp_only_differ_on_mask:
+  assumes "ctxt, StateCons, \<omega>def_opt \<turnstile> \<langle>e; \<omega>\<rangle> [\<Down>]\<^sub>t Val v"
+      and "no_perm_pure_exp e \<and> no_unfolding_pure_exp e"
+      and "get_h_total_full \<omega> = get_h_total_full \<omega>'"
+      and "get_store_total \<omega> = get_store_total \<omega>'"
+      and "get_trace_total \<omega> = get_trace_total \<omega>'"
+  shows "ctxt, StateCons, \<omega>def_opt \<turnstile> \<langle>e; \<omega>'\<rangle> [\<Down>]\<^sub>t Val v"
+  sorry
+
+lemma red_pure_exp_different_def_state:
+  assumes "ctxt, StateCons, \<omega>def_opt \<turnstile> \<langle>e; \<omega>\<rangle> [\<Down>]\<^sub>t Val v"
+      and "no_perm_pure_exp e \<and> no_unfolding_pure_exp e"
+    shows "ctxt, StateCons, \<omega>def_opt' \<turnstile> \<langle>e; \<omega>\<rangle> [\<Down>]\<^sub>t Val v \<or> ctxt, StateCons, \<omega>def_opt' \<turnstile> \<langle>e; \<omega>\<rangle> [\<Down>]\<^sub>t VFailure"
+  sorry
+  
+lemma exhale_inhale_normal:
+  assumes RedExh: "red_exhale ctxt StateCons \<omega>def A \<omega> res" 
+      and "res = RNormal \<omega>'"
+      and "mono_prop_downward StateCons"
+      and "no_perm_assertion A \<and> no_unfolding_assertion A"
+      and "assertion_framing_state ctxt StateCons A \<omega>_inh"
+      and "\<omega>_inh \<oplus> (\<omega> \<ominus> \<omega>') = Some \<omega>_inh'"
+      and ValidInh':"StateCons \<omega>_inh' \<and> valid_heap_mask (get_mh_total_full \<omega>_inh')"
+    shows "red_inhale ctxt StateCons A \<omega>_inh (RNormal \<omega>_inh')"
+  using assms exhale_normal_result_smaller[OF RedExh[simplified \<open>res = _\<close>]]
+proof (induction arbitrary: \<omega>_inh \<omega>_inh' \<omega>')
+  case (ExhAcc mh \<omega> e_r r e_p p a f)
+  let ?A = "(Acc e_r f (PureExp e_p))"
+  note AssertionFramed = \<open>assertion_framing_state ctxt StateCons (Atomic (Acc e_r f (PureExp e_p))) \<omega>_inh\<close>
+
+  have SubExp: "sub_expressions_atomic ?A = [e_r, e_p]"
+    by simp
+
+  from \<open>\<omega>_inh \<oplus> (\<omega> \<ominus> \<omega>') = Some \<omega>_inh'\<close> and \<open>\<omega> \<succeq> \<omega>'\<close> have 
+    OnlyMaskChanged:
+    "get_store_total \<omega>_inh = get_store_total \<omega> \<and>
+     get_trace_total \<omega>_inh = get_trace_total \<omega> \<and>
+     get_h_total_full \<omega>_inh = get_h_total_full \<omega>"
+    by (metis full_total_state_greater_only_mask_changed greater_def greater_equiv minus_smaller)
+
+
+  have "ctxt, StateCons, Some \<omega>_inh \<turnstile> \<langle>e_r;\<omega>_inh\<rangle> [\<Down>]\<^sub>t Val (VRef r)" (is ?RedRefInh)
+  proof (rule ccontr)
+    from OnlyMaskChanged ExhAcc have
+       RedRefAux: "ctxt, StateCons, Some \<omega>def \<turnstile> \<langle>e_r;\<omega>_inh\<rangle> [\<Down>]\<^sub>t Val (VRef r)"
+    using red_pure_exp_only_differ_on_mask
+    by fastforce
+
+    assume "\<not>?RedRefInh"
+    moreover have "ctxt, StateCons, Some \<omega>_inh \<turnstile> \<langle>e_r;\<omega>_inh\<rangle> [\<Down>]\<^sub>t (Val (VRef r)) \<or>
+          ctxt, StateCons, Some \<omega>_inh \<turnstile> \<langle>e_r;\<omega>_inh\<rangle> [\<Down>]\<^sub>t VFailure"
+      using red_pure_exp_different_def_state[OF RedRefAux] ExhAcc
+      by simp
+    ultimately show False
+      using AssertionFramed SubExp
+      unfolding assertion_framing_state_def
+      by (metis InhSubAtomicFailure RedExpListFailure list.distinct(1))
+  qed
+
+  have "ctxt, StateCons, Some \<omega>_inh \<turnstile> \<langle>e_p;\<omega>_inh\<rangle> [\<Down>]\<^sub>t Val (VPerm p)" (is ?RedPermInh)
+  proof (rule ccontr)
+    from OnlyMaskChanged ExhAcc have
+       Aux: "ctxt, StateCons, Some \<omega>def \<turnstile> \<langle>e_p;\<omega>_inh\<rangle> [\<Down>]\<^sub>t Val (VPerm p)"
+    using red_pure_exp_only_differ_on_mask
+    by fastforce
+
+    assume "\<not>?RedPermInh"
+    moreover have *: "ctxt, StateCons, Some \<omega>_inh \<turnstile> \<langle>e_p;\<omega>_inh\<rangle> [\<Down>]\<^sub>t (Val (VPerm p)) \<or>
+          ctxt, StateCons, Some \<omega>_inh \<turnstile> \<langle>e_p;\<omega>_inh\<rangle> [\<Down>]\<^sub>t VFailure"
+      using red_pure_exp_different_def_state[OF Aux] ExhAcc
+      by simp
+
+    moreover have "red_inhale ctxt StateCons (Atomic ?A) \<omega>_inh RFailure"
+    proof -
+      from * \<open>\<not>?RedPermInh\<close> have "ctxt, StateCons, Some \<omega>_inh \<turnstile> \<langle>e_p;\<omega>_inh\<rangle> [\<Down>]\<^sub>t VFailure"
+        by blast
+
+      thus ?thesis
+        using \<open>?RedRefInh\<close> InhSubAtomicFailure TotalExpressions.RedExpListCons RedExpListFailure
+        by (metis None_eq_map_option_iff SubExp neq_Nil_conv)
+    qed
+
+    ultimately show False
+      using AssertionFramed 
+      unfolding assertion_framing_state_def
+      by blast
+  qed
+      
+  show ?case
+  proof (cases "r = Null")
+    case True
+    hence "\<omega> = \<omega>'"
+      using ExhAcc(5)
+      by (simp add: exh_if_total_normal_2)
+
+    have "\<omega>_inh' = \<omega>_inh"
+      using \<open>\<omega>_inh \<oplus> (\<omega> \<ominus> \<omega>') = Some \<omega>_inh'\<close>[simplified \<open>\<omega> = \<omega>'\<close>]
+            full_total_state_defined_core_same_2 plus_minus_empty
+      by (metis option.sel)
+
+    show ?thesis
+      apply (rule InhAcc[OF \<open>?RedRefInh\<close> \<open>?RedPermInh\<close>])
+       apply simp
+      using \<open>\<omega>_inh' = \<omega>_inh\<close> \<open>r = Null\<close> ExhAcc.prems(1) THResultNormal \<open>\<omega> = \<omega>'\<close> exh_if_total_normal 
+      by fastforce
+  next
+    case False
+    from this obtain a where "r = Address a"
+      using ref.exhaust by blast    
+
+    hence PermConditions: "0 \<le> p \<and> pgte (mh (a, f)) (Abs_prat p)"
+      using ExhAcc.hyps(4) ExhAcc.prems(1) exh_if_total_normal by fastforce
+
+    from \<open>r = Address a\<close> have "\<omega>' = update_mh_loc_total_full \<omega> (a, f) (mh (a, f) - Abs_prat p)"
+      using ExhAcc.hyps(4) ExhAcc.prems(1) exh_if_total_normal_2 by auto
+
+    let ?m\<Delta> = "\<lambda>loc. if loc = (a,f) then (Abs_prat p) else pnone"
+
+    let ?p' = "(padd (get_mh_total_full \<omega>_inh (a,f)) (Abs_prat p))"
+    have "\<omega>_inh' = update_mh_loc_total_full \<omega>_inh (a,f) ?p'" (is "_ = ?upd_\<omega>_inh")        
+
+    proof -
+      from \<open>\<omega>_inh \<oplus> (\<omega> \<ominus> \<omega>') = Some \<omega>_inh'\<close>
+      have "\<omega>_inh' = update_m_total_full \<omega>_inh (add_masks (get_mh_total_full \<omega>_inh) (get_mh_total_full (\<omega> \<ominus> \<omega>')))
+                                               (add_masks (get_mp_total_full \<omega>_inh) (get_mp_total_full (\<omega> \<ominus> \<omega>')))"
+        using plus_Some_full_total_state_eq
+        by blast
+      moreover have "(add_masks (get_mp_total_full \<omega>_inh) (get_mp_total_full (\<omega> \<ominus> \<omega>'))) = (get_mp_total_full \<omega>_inh)"
+      proof -
+        have "get_mp_total_full (\<omega> \<ominus> \<omega>') = zero_mask"
+          apply (simp only: minus_full_total_state_mask[OF \<open>\<omega> \<succeq> \<omega>'\<close>])
+          by (simp add: \<open>\<omega>' = _\<close> minus_masks_empty)
+
+        thus ?thesis
+          by (simp add: add_masks_zero_mask)
+      qed
+      moreover have "add_masks (get_mh_total_full \<omega>_inh) (get_mh_total_full (\<omega> \<ominus> \<omega>')) =  
+                               (get_mh_total_full \<omega>_inh)( (a,f) := ?p')" (is "?lhs = ?rhs")
+      proof -
+        have *: "get_mh_total_full (\<omega> \<ominus> \<omega>') = get_mh_total_full \<omega> - (get_mh_total_full \<omega>)( (a,f) := (get_mh_total_full \<omega> (a, f) - Abs_prat p))"
+          apply (simp only: minus_full_total_state_mask[OF \<open>\<omega> \<succeq> \<omega>'\<close> ])
+          by (simp add: \<open>\<omega>' =_\<close> \<open>mh = _\<close>)
+
+        show ?thesis
+          unfolding add_masks_def
+        proof (subst *, standard)
+          fix hl
+          let ?mh_inh = "get_mh_total_full \<omega>_inh"
+          let ?mh = "get_mh_total_full \<omega>"
+
+          show "padd (?mh_inh hl) ((?mh - ?mh((a, f) := ?mh (a, f) - Abs_prat p)) hl) =
+                     (?mh_inh((a, f) := padd (?mh_inh (a, f)) (Abs_prat p))) hl"
+          proof (cases "hl = (a,f)")
+            case True
+            then show ?thesis 
+              using PermConditions[simplified \<open>mh = _\<close>, THEN HOL.conjunct2, THEN minus_prat_gte]
+              by simp
+          next
+            case False
+            then show ?thesis
+              using zero_prat_def
+              by (simp add: minus_prat_def)
+          qed
+        qed
+      qed
+
+      ultimately show ?thesis
+        by simp
+    qed        
+
+    hence "get_mh_total_full \<omega>_inh' (a,f) = (padd (get_mh_total_full \<omega>_inh (a,f)) (Abs_prat p))"
+      by simp
+
+    hence PermConstraint': "pgte pwrite (padd (get_mh_total_full \<omega>_inh (a, f)) (Abs_prat p))"
+      using ExhAcc.prems(6)
+      unfolding valid_heap_mask_def
+      by metis
+      
+    let ?W = "inhale_perm_single StateCons \<omega>_inh (a, f) (Some (Abs_prat p))"
+
+    have "\<omega>_inh' \<in> ?W"
+      unfolding inhale_perm_single_def
+      apply (rule Set.CollectI)
+      apply (rule exI)+
+      apply (intro conjI)
+          apply simp
+      using ExhAcc
+         apply blast
+        apply simp
+       apply (rule PermConstraint')
+      apply (simp add: \<open>\<omega>_inh' = _\<close>)
+      done
+      
+      show ?thesis        
+       apply (rule InhAcc[OF \<open>?RedRefInh\<close> \<open>?RedPermInh\<close>])
+       apply simp
+      using PermConditions \<open>\<omega>_inh' \<in> ?W\<close>
+      by (smt (verit) False Set.set_insert THResultNormal \<open>r = Address a\<close> insert_not_empty ref.sel)
+  qed
+next
+  case (ExhAccWildcard mh \<omega> e_r r q a f)
+  then show ?case sorry
+next
+  case (ExhAccPred mp \<omega> e_args v_args e_p p pred_id r)
+  then show ?case sorry
+next
+  case (ExhAccPredWildcard mp \<omega> e_args v_args q a f pred_id)
+  then show ?case sorry
+next
+  case (ExhPure e \<omega> b)
+  hence "b = True"
+    using exh_if_total_normal exh_if_total_normal_2 by blast
+
+  from ExhPure have "\<omega>' = \<omega>"
+    by (auto elim: exh_if_total.elims)
+  hence "\<omega>_inh' = \<omega>_inh"
+    using \<open>\<omega>_inh \<oplus> (\<omega> \<ominus> \<omega>') = Some \<omega>_inh'\<close>
+    by (metis full_total_state_defined_core_same_2 option.inject plus_minus_empty)
+
+  note OnlyMaskChanged = minus_full_total_state_only_mask_different_2[OF \<open>\<omega>_inh \<oplus> (\<omega> \<ominus> \<omega>') = Some \<omega>_inh'\<close>]
+  with ExhPure have RedAux: "ctxt, StateCons, Some \<omega>def \<turnstile> \<langle>e;\<omega>_inh\<rangle> [\<Down>]\<^sub>t Val (VBool True)"    
+    using red_pure_exp_only_differ_on_mask
+    unfolding \<open>b = True\<close>
+    by fastforce
+
+  have "ctxt, StateCons, Some \<omega>_inh \<turnstile> \<langle>e;\<omega>_inh\<rangle> [\<Down>]\<^sub>t Val (VBool True)"
+  proof -
+    have "\<not> ctxt, StateCons, Some \<omega>_inh \<turnstile> \<langle>e;\<omega>_inh\<rangle> [\<Down>]\<^sub>t VFailure"
+      using \<open>assertion_framing_state ctxt StateCons (Atomic (Pure e)) \<omega>_inh\<close>
+      unfolding assertion_framing_state_def
+      by (metis (no_types, opaque_lifting) InhSubAtomicFailure RedExpListFailure not_None_eq red_exp_list_failure_Nil sub_expressions_atomic.simps(1))
+
+    thus ?thesis
+      using red_pure_exp_different_def_state[OF RedAux] ExhPure
+      by auto
+  qed
+
+  then show ?case
+    by (auto intro: inh_pure_normal simp: \<open>\<omega>_inh' = \<omega>_inh\<close>)
+next
+  case (SubAtomicFailure A \<omega>)
+  then show ?case by simp \<comment>\<open>contradiction\<close>
+next
+  case (ExhStarNormal A \<omega> \<omega>'' B res)
+  hence "\<omega> \<succeq> \<omega>''" and "\<omega>'' \<succeq> \<omega>'"
+    by (simp_all add: exhale_normal_result_smaller)
+
+  note AssertionFraming = \<open>assertion_framing_state ctxt StateCons (A && B) \<omega>_inh\<close>
+  hence AssertionFramingA: "assertion_framing_state ctxt StateCons A \<omega>_inh"
+    using assertion_framing_star
+    by blast
+
+  from ExhStarNormal have ConstraintA: "no_perm_assertion A \<and> no_unfolding_assertion A" and
+                          ConstraintB: "no_perm_assertion B \<and> no_unfolding_assertion B"
+    by simp_all
+
+  have "\<omega> \<ominus> \<omega>' \<succeq> \<omega> \<ominus> \<omega>''"
+    using \<open>\<omega>'' \<succeq> \<omega>'\<close> \<open>\<omega> \<succeq> \<omega>''\<close> minus_greater
+    by blast
+
+  moreover from this obtain \<omega>_inh'' where \<omega>_inh''_Some: "\<omega>_inh \<oplus> (\<omega> \<ominus> \<omega>'') = Some \<omega>_inh''"
+    using \<open>\<omega>_inh \<oplus> (\<omega> \<ominus> \<omega>') = Some \<omega>_inh'\<close> 
+    by (metis commutative compatible_smaller)
+
+  ultimately have "\<omega>_inh' \<succeq> \<omega>_inh''"
+    using \<open>\<omega>_inh \<oplus> (\<omega> \<ominus> \<omega>') = Some \<omega>_inh'\<close>
+    by (metis (full_types) addition_bigger commutative)
+    
+  hence \<omega>_inh''_valid: "StateCons \<omega>_inh'' \<and> valid_heap_mask (get_mh_total_full \<omega>_inh'')"
+    using \<open>StateCons \<omega>_inh' \<and> valid_heap_mask (get_mh_total_full \<omega>_inh')\<close> 
+          \<open>mono_prop_downward StateCons\<close>[simplified mono_prop_downward_def] valid_heap_mask_downward_mono
+          full_total_state_greater_mask 
+    by blast
+    
+  have RedInhA: "red_inhale ctxt StateCons A \<omega>_inh (RNormal \<omega>_inh'')"
+    using ExhStarNormal.IH(1)[OF _ \<open>mono_prop_downward StateCons\<close> ConstraintA AssertionFramingA \<omega>_inh''_Some \<omega>_inh''_valid] ExhStarNormal.prems
+          \<open>\<omega> \<succeq> \<omega>''\<close>
+    by simp
+
+  with AssertionFraming have AssertionFramingB: "assertion_framing_state ctxt StateCons B \<omega>_inh''"
+    using assertion_framing_star
+    by blast
+
+  have \<omega>_inh'_Some2: "\<omega>_inh'' \<oplus> (\<omega>'' \<ominus> \<omega>') = Some \<omega>_inh'"
+    using \<omega>_inh''_Some \<open>\<omega>_inh \<oplus> (\<omega> \<ominus> \<omega>') = Some \<omega>_inh'\<close> \<open>\<omega>'' \<succeq> \<omega>'\<close>
+    by (smt (z3) \<open>\<omega> \<succeq> \<omega>''\<close> asso1 commutative minus_and_plus minus_equiv_def)
+
+  have "red_inhale ctxt StateCons B \<omega>_inh'' (RNormal \<omega>_inh')"
+  using ExhStarNormal.IH(2)[OF _ \<open>mono_prop_downward StateCons\<close> ConstraintB AssertionFramingB \<omega>_inh'_Some2 ] ExhStarNormal.prems
+          \<open>\<omega>'' \<succeq> \<omega>'\<close>
+  by simp
+
+  then show ?case 
+  using RedInhA
+  by (fastforce intro: InhStarNormal)    
+next
+  case (ExhStarFailure A \<omega> B)
+  then show ?case by simp \<comment>\<open>contradiction\<close>
+next
+  case (ExhImpTrue e \<omega> A res)
+  with minus_full_total_state_only_mask_different_2[OF \<open>\<omega>_inh \<oplus> (\<omega> \<ominus> \<omega>') = Some \<omega>_inh'\<close>]
+  have RedAux: "ctxt, StateCons, Some \<omega>def \<turnstile> \<langle>e;\<omega>_inh\<rangle> [\<Down>]\<^sub>t Val (VBool True)"    
+    using red_pure_exp_only_differ_on_mask
+    by fastforce
+
+  note AssertionFraming = \<open>assertion_framing_state ctxt StateCons (assert.Imp e A) \<omega>_inh\<close>
+
+  have RedExpInh: "ctxt, StateCons, Some \<omega>_inh \<turnstile> \<langle>e;\<omega>_inh\<rangle> [\<Down>]\<^sub>t Val (VBool True)"
+  proof -
+    have "\<not> ctxt, StateCons, Some \<omega>_inh \<turnstile> \<langle>e;\<omega>_inh\<rangle> [\<Down>]\<^sub>t VFailure"
+      using AssertionFraming
+      unfolding assertion_framing_state_def
+      using InhImpFailure by blast
+
+    thus ?thesis
+      using red_pure_exp_different_def_state[OF RedAux] ExhImpTrue
+      by auto
+  qed
+
+  hence "assertion_framing_state ctxt StateCons A \<omega>_inh"
+    using assertion_framing_imp AssertionFraming
+    by blast
+
+  hence "red_inhale ctxt StateCons A \<omega>_inh (RNormal \<omega>_inh')"
+    using ExhImpTrue
+    by auto
+
+  thus ?case
+    using RedExpInh
+    by (auto intro: red_inhale_intros)  
+next
+  case (ExhImpFalse e \<omega> A)
+  hence "\<omega>_inh' = \<omega>_inh"
+    by (metis full_total_state_defined_core_same_2 option.inject plus_minus_empty stmt_result_total.inject)
+
+  have "ctxt, StateCons, Some \<omega>_inh \<turnstile> \<langle>e;\<omega>_inh\<rangle> [\<Down>]\<^sub>t Val (VBool False)"
+  proof -
+    have RedAux: "ctxt, StateCons, Some \<omega>def \<turnstile> \<langle>e;\<omega>_inh\<rangle> [\<Down>]\<^sub>t Val (VBool False)"
+      using ExhImpFalse minus_full_total_state_only_mask_different_2[OF \<open>\<omega>_inh \<oplus> (\<omega> \<ominus> \<omega>') = Some \<omega>_inh'\<close>]
+            red_pure_exp_only_differ_on_mask
+      by fastforce
+
+    have "\<not> (ctxt, StateCons, Some \<omega>_inh \<turnstile> \<langle>e;\<omega>_inh\<rangle> [\<Down>]\<^sub>t VFailure)"
+      using \<open>assertion_framing_state ctxt StateCons (assert.Imp e A) \<omega>_inh\<close> InhImpFailure
+      unfolding assertion_framing_state_def
+      by blast
+
+    thus ?thesis
+      using red_pure_exp_different_def_state[OF RedAux] ExhImpFalse
+      by auto
+  qed            
+
+  then show ?case 
+    by (auto intro: red_inhale_intros simp: \<open>\<omega>_inh' = \<omega>_inh\<close>)  
+next
+  case (ExhImpFailure e \<omega> A)
+  then show ?case by simp \<comment>\<open>contradiction\<close>
+qed
+
 
 subsection \<open>Unfold leads to one normal successor state\<close>
 
